Main.lean
@@ -110,6 +110,46 @@ by
   | ok u =>
     simp
 
+def checkValidnessGraphMockDatabase {helper: parsingArityHelper} (problem: graphVerificationProblem helper):  Except String Unit :=
+  let m:= parseProgramToSymbolSequenceMap problem.program (fun _ => [])
+  let d:= mockDatabase (parsingSignature helper)
+  dfs problem.graph (fun a l => locallyValidityChecker m d l a ruleParsingSignatureToString)
+
+lemma checkValidnessGraphMockDatabaseIffAllValid {helper: parsingArityHelper}  (problem: graphVerificationProblem helper): checkValidnessGraphMockDatabase problem = Except.ok () ↔ isAcyclic problem.graph ∧ (∀ (a:groundAtom (parsingSignature helper) ), a ∈ problem.graph.vertices → locallyValid problem.program.toFinset (mockDatabase (parsingSignature helper)) a problem.graph) ∧ problem.graph.vertices.toSet ⊆ proofTheoreticSemantics problem.program.toFinset (mockDatabase (parsingSignature helper)) :=
+by
+  unfold checkValidnessGraphMockDatabase
+  rw [dfs_semantics]
+  constructor
+  intro h
+  rcases h with ⟨acyc, localValid⟩
+  constructor
+  apply acyc
+  constructor
+  intro a a_mem
+  specialize localValid a a_mem
+  rw [locallyValidityCheckerUnitIffLocallyValid (P:=problem.program) (G:=problem.graph)] at localValid
+  apply localValid
+  rfl
+  rfl
+  apply verticesOfLocallyValidAcyclicGraphAreInProofTheoreticSemantics (acyclic:=acyc)
+  intro a a_mem
+  specialize localValid a a_mem
+  rw [locallyValidityCheckerUnitIffLocallyValid (P:=problem.program) (G:=problem.graph)] at localValid
+  apply localValid
+  rfl
+  rfl
+
+  intro h
+  rcases h with ⟨acyclic, valid, _ ⟩
+  constructor
+  apply acyclic
+  intro a a_mem
+  rw [locallyValidityCheckerUnitIffLocallyValid (P:=problem.program) (G:=problem.graph)]
+  apply valid a a_mem
+  rfl
+  rfl
+
+
 
 def mainCheckMockDatabase {helper: parsingArityHelper} (problem: verificationProblem helper) (safe: ∀ (r: rule (parsingSignature helper) ), r ∈ problem.program → r.isSafe): Except String Unit :=
   let d:= mockDatabase (parsingSignature helper)
@@ -124,13 +164,13 @@ def mainCheckMockDatabase {helper: parsingArityHelper} (problem: verificationPro
       then Except.ok ()
       else Except.error "Model does not contain database"
 
-lemma mainCheckMockDatabseUnitIffSolution  (problem: verificationProblem relationList) (safe: ∀ (r: rule (parsingSignature relationList) ), r ∈ problem.program → r.isSafe): mainCheckMockDatabase problem safe = Except.ok () ↔ (List.toSet (collectModel problem.trees)) = proofTheoreticSemantics problem.program.toFinset (mockDatabase (parsingSignature relationList)) ∧ ∀ (t: proofTree (parsingSignature relationList)), t ∈ problem.trees → isValid problem.program.toFinset (mockDatabase (parsingSignature relationList)) t:= by
+lemma mainCheckMockDatabaseUnitIffSolution {helper: parsingArityHelper}  (problem: verificationProblem helper) (safe: ∀ (r: rule (parsingSignature helper) ), r ∈ problem.program → r.isSafe): mainCheckMockDatabase problem safe = Except.ok () ↔ (List.toSet (collectModel problem.trees)) = proofTheoreticSemantics problem.program.toFinset (mockDatabase (parsingSignature helper)) ∧ ∀ (t: proofTree (parsingSignature helper)), t ∈ problem.trees → isValid problem.program.toFinset (mockDatabase (parsingSignature helper)) t:= by
   constructor
   unfold mainCheckMockDatabase
   simp
   intro h
 
-  cases valid_trees: validateTreeList problem.program (mockDatabase (parsingSignature relationList)) problem.trees
+  cases valid_trees: validateTreeList problem.program (mockDatabase (parsingSignature helper)) problem.trees
    ruleParsingSignatureToString with
   | error e => simp [valid_trees] at h
   | ok _ =>
@@ -152,7 +192,7 @@ lemma mainCheckMockDatabseUnitIffSolution  (problem: verificationProblem relatio
       constructor
       apply model
       rw [← mockDatabaseContainedInModelTrue]
-      have db: mockDatabaseContainedInModel (mockDatabase (parsingSignature relationList)) (List.toSet (collectModel problem.trees)) = true
+      have db: mockDatabaseContainedInModel (mockDatabase (parsingSignature helper)) (List.toSet (collectModel problem.trees)) = true
       by_contra p
       simp at p
       specialize h p
@@ -164,7 +204,7 @@ lemma mainCheckMockDatabseUnitIffSolution  (problem: verificationProblem relatio
   rcases h with ⟨sol_eq, valid_tree⟩
   unfold mainCheckMockDatabase
   simp
-  have p: validateTreeList problem.program (mockDatabase (parsingSignature relationList)) problem.trees ruleParsingSignatureToString = Except.ok ()
+  have p: validateTreeList problem.program (mockDatabase (parsingSignature helper)) problem.trees ruleParsingSignatureToString = Except.ok ()
   rw [validateTreeListUnitIffSubsetSemanticsAndAllElementsHaveValidTrees]
   constructor
   rw [← collectModelToSetIsSetOfValidTreesElements]
@@ -172,7 +212,7 @@ lemma mainCheckMockDatabseUnitIffSolution  (problem: verificationProblem relatio
   apply valid_tree
 
   simp [p]
-  have model: model (List.toFinset problem.program) (mockDatabase (parsingSignature relationList)) (List.toSet (collectModel problem.trees))
+  have model: model (List.toFinset problem.program) (mockDatabase (parsingSignature helper)) (List.toSet (collectModel problem.trees))
   rw [sol_eq]
   apply proofTheoreticSemanticsIsModel
   unfold model at model
@@ -186,10 +226,106 @@ lemma mainCheckMockDatabseUnitIffSolution  (problem: verificationProblem relatio
   unfold mockDatabaseContainedInModel
   simp
 
+
+def mainCheckGraphMockDatabase {helper: parsingArityHelper} (problem: graphVerificationProblem helper) (safe: ∀ (r: rule (parsingSignature helper) ), r ∈ problem.program → r.isSafe): Except String Unit :=
+  let m:= parseProgramToSymbolSequenceMap problem.program (fun _ => [])
+  let d:= mockDatabase (parsingSignature helper)
+  match dfs problem.graph (fun a l => locallyValidityChecker m d l a ruleParsingSignatureToString)   with
+  | Except.error e => Except.error e
+  | Except.ok _ =>
+    match modelChecker problem.graph.vertices problem.program safe with
+    | Except.error e => Except.error e
+    | Except.ok _ =>
+      if mockDatabaseContainedInModel d (List.toSet problem.graph.vertices) = true
+      then Except.ok ()
+      else Except.error "Model does not contain database"
+
+lemma mainCheckGraphMockDatabaseUnitIffSolution {helper: parsingArityHelper} (problem: graphVerificationProblem helper) (safe: ∀ (r: rule (parsingSignature helper) ), r ∈ problem.program → r.isSafe): mainCheckGraphMockDatabase problem safe = Except.ok () ↔ (List.toSet problem.graph.vertices) = proofTheoreticSemantics problem.program.toFinset (mockDatabase (parsingSignature helper)) ∧ isAcyclic problem.graph ∧ (∀ (a:groundAtom (parsingSignature helper) ), a ∈ problem.graph.vertices → locallyValid problem.program.toFinset (mockDatabase (parsingSignature helper)) a problem.graph):=
+by
+  unfold mainCheckGraphMockDatabase
+  simp
+  constructor
+  intro h
+  simp at h
+  cases dfs_result: dfs problem.graph (fun a l => locallyValidityChecker (parseProgramToSymbolSequenceMap problem.program (fun _ => [])) (mockDatabase (parsingSignature helper)) l a ruleParsingSignatureToString )with
+  | error e =>
+    simp[dfs_result] at h
+  | ok _ =>
+    simp [dfs_result] at h
+    cases modelCheck: modelChecker problem.graph.vertices problem.program safe with
+    | error e =>
+      simp [modelCheck] at h
+    | ok _ =>
+      simp only [modelCheck] at h
+      have db: mockDatabaseContainedInModel (mockDatabase (parsingSignature helper)) (List.toSet problem.graph.vertices) = true
+      by_contra p
+      simp [p] at h
+
+      rw [dfs_semantics] at dfs_result
+      rcases dfs_result with ⟨acyclic,valid⟩
+      rw [modelCheckerUnitIffAllRulesTrue] at modelCheck
+      rw [mockDatabaseContainedInModelTrue] at db
+      constructor
+      apply Set.Subset.antisymm
+      apply verticesOfLocallyValidAcyclicGraphAreInProofTheoreticSemantics _ _ _ acyclic
+      intro a a_mem
+      specialize valid a a_mem
+      rw [locallyValidityCheckerUnitIffLocallyValid (P:=problem.program) (G:=problem.graph)] at valid
+      apply valid
+      rfl
+      rfl
+
+      rw [SemanticsEquivalence]
+      apply leastModel
+      unfold model
+      constructor
+      apply modelCheck
+      apply db
+
+      --end semantics
+      constructor
+      apply acyclic
+      intro a a_mem
+      specialize valid a a_mem
+      rw [locallyValidityCheckerUnitIffLocallyValid (P:=problem.program) (G:=problem.graph)] at valid
+      apply valid
+      rfl
+      rfl
+
+  intro h
+  rcases h with ⟨semantics, acyclic, valid⟩
+  have dfs_result: dfs problem.graph (fun a l =>
+      locallyValidityChecker (parseProgramToSymbolSequenceMap problem.program fun _ => [])
+        (mockDatabase (parsingSignature helper)) l a ruleParsingSignatureToString) = Except.ok ()
+  rw [dfs_semantics]
+  constructor
+  apply acyclic
+  intro a a_mem
+  rw [locallyValidityCheckerUnitIffLocallyValid (P:=problem.program) (G:=problem.graph)]
+  apply valid a a_mem
+  rfl
+  rfl
+  simp [dfs_result]
+
+  have modelChecker: modelChecker problem.graph.vertices problem.program safe = Except.ok ()
+  rw [modelCheckerUnitIffAllRulesTrue]
+  intro r rP
+  have ismodel: model problem.program.toFinset (mockDatabase (parsingSignature helper)) (List.toSet problem.graph.vertices)
+  rw [semantics]
+  apply proofTheoreticSemanticsIsModel
+  unfold model at ismodel
+  apply And.left ismodel r rP
+  simp only [modelChecker]
+
+  unfold mockDatabaseContainedInModel
+  simp
+
+
 structure argsParsed where
   (programFileName: String)
   (complete: Bool)
   (help: Bool)
+  (graph: Bool)
 
 def parseArgsHelper (args: List String) (curr: argsParsed) : Except String argsParsed  :=
   match args with
@@ -199,15 +335,21 @@ def parseArgsHelper (args: List String) (curr: argsParsed) : Except String argsP
     else Except.ok curr
   | hd::tl =>
     if hd ∈ ["-h", "--help"]
-    then Except.ok {programFileName := "", complete := false, help := true}
-    else  if hd == "-c"
-          then parseArgsHelper tl {programFileName := "", complete := true, help := false}
+    then Except.ok {programFileName := "", complete := false, help := true, graph:= false}
+    else  if hd ∈  ["-c", "-g"]
+          then
+            if hd == "-c"
+            then parseArgsHelper tl {programFileName := "", complete := true, help := false, graph:= curr.graph}
+            else
+              if hd == "-g"
+              then  parseArgsHelper tl {programFileName := "", complete := curr.complete , help := false, graph:= true}
+              else Except.error ("Unknown argument " ++ hd)
           else
           if tl == []
-          then Except.ok {programFileName := hd, complete := curr.complete, help := false}
+          then Except.ok {programFileName := hd, complete := curr.complete, help := false, graph:= curr.graph}
           else Except.error "Too many arguments"
 
-def parseArgs (args: List String): Except String argsParsed := parseArgsHelper args {programFileName := "", complete := false, help:= false}
+def parseArgs (args: List String): Except String argsParsed := parseArgsHelper args {programFileName := "", complete := false, help:= false, graph:= false}
 
 def printHelp: IO Unit := do
   IO.println "Datalog results validity checker"
@@ -216,9 +358,10 @@ def printHelp: IO Unit := do
   IO.println "  <problemFile>: contains a json description of the program and the proof trees"
   IO.println "Options"
   IO.println "  -h --help Help (displayed right now)"
+  IO.println "  -g        Use a graph instead of a list of trees as an input via a list of edges (start -- end)"
   IO.println "  -c        Completeness check: in addition to validating the trees check if result is also a model"
 
-def getProblemFromJson (fileName: String): IO (Except String (verificationProblemSignatureWrapper)) := do
+def getTreeProblemFromJson (fileName: String): IO (Except String (verificationProblemSignatureWrapper)) := do
   let filePath := System.FilePath.mk fileName
   if ← filePath.pathExists
       then
@@ -228,8 +371,67 @@ def getProblemFromJson (fileName: String): IO (Except String (verificationProble
             match Lean.fromJson? (α:=problemInput) json with
               | Except.error msg => pure (Except.error ("Json does not match problem description" ++ msg))
               | Except.ok parsedProblem =>
-                pure (converProblemInputToVerificationProblem parsedProblem)
+                pure (convertProblemInputToVerificationProblem parsedProblem)
   else pure (Except.error "File does not exist")
+
+def main_trees (argsParsed: argsParsed): IO Unit := do
+  match ← getTreeProblemFromJson argsParsed.programFileName with
+  | Except.error e => IO.println e
+  | Except.ok transformedInput =>
+    let problem := transformedInput.problem
+    if argsParsed.complete = true
+    then
+      IO.println "Completeness check"
+      match safe: safetyCheckProgram problem.program ruleParsingSignatureToString (fun x => x) with
+      | Except.error msg => IO.println msg
+      | Except.ok _ =>
+        have safe': ∀ (r: rule (parsingSignature transformedInput.helper)), r ∈ problem.program → r.isSafe := by
+          rw [safetyCheckProgramUnitIffProgramSafe] at safe
+          apply safe
+        match mainCheckMockDatabase problem safe' with
+        | Except.ok _ => IO.println "Valid result"
+        | Except.error msg => IO.println ("Invalid result due to " ++ msg )
+    else
+      match checkValidnessMockDatabase problem with
+      | Except.error msg => IO.println ("Invalid result due to " ++ msg )
+      | Except.ok _ => IO.println "Valid result"
+
+def getGraphProblemFromJson (fileName: String): IO (Except String (graphVerificationProblemSignatureWrapper)) := do
+  let filePath := System.FilePath.mk fileName
+  if ← filePath.pathExists
+      then
+        match Lean.Json.parse (← IO.FS.readFile filePath) with
+          | Except.error msg => pure (Except.error ("Error parsing JSON " ++ msg))
+          | Except.ok json =>
+            match Lean.fromJson? (α:=graphInputProblem) json with
+              | Except.error msg => pure (Except.error ("Json does not match problem description" ++ msg))
+              | Except.ok parsedProblem =>
+                pure (convertGraphProblemInputToGraphVerificationProblem parsedProblem)
+  else pure (Except.error "File does not exist")
+
+
+def main_graph (argsParsed: argsParsed): IO Unit := do
+  match ← getGraphProblemFromJson argsParsed.programFileName with
+  | Except.error e => IO.println e
+  | Except.ok transformedInput =>
+    let problem := transformedInput.problem
+    if argsParsed.complete = true
+    then
+      IO.println "Completeness check"
+      match safe: safetyCheckProgram problem.program ruleParsingSignatureToString (fun x => x) with
+      | Except.error msg => IO.println msg
+      | Except.ok _ =>
+        have safe': ∀ (r: rule (parsingSignature transformedInput.helper)), r ∈ problem.program → r.isSafe := by
+          rw [safetyCheckProgramUnitIffProgramSafe] at safe
+          apply safe
+        match mainCheckGraphMockDatabase problem safe' with
+        | Except.ok _ => IO.println "Valid result"
+        | Except.error msg => IO.println ("Invalid result due to " ++ msg )
+    else
+      match checkValidnessGraphMockDatabase problem with
+      | Except.error msg => IO.println ("Invalid result due to " ++ msg )
+      | Except.ok _ => IO.println "Valid result"
+
 
 def main(args: List String): IO Unit := do
   match parseArgs args with
@@ -238,23 +440,8 @@ def main(args: List String): IO Unit := do
     if argsParsed.help = true
     then printHelp
     else
-      match ← getProblemFromJson argsParsed.programFileName with
-      | Except.error e => IO.println e
-      | Except.ok transformedInput =>
-        let problem := transformedInput.problem
-        if argsParsed.complete = true
-        then
-          IO.println "Completeness check"
-          match safe: safetyCheckProgram problem.program ruleParsingSignatureToString (fun x => x) with
-          | Except.error msg => IO.println msg
-          | Except.ok _ =>
-            have safe': ∀ (r: rule (parsingSignature transformedInput.helper)), r ∈ problem.program → r.isSafe := by
-              rw [safetyCheckProgramUnitIffProgramSafe] at safe
-              apply safe
-            match mainCheckMockDatabase problem safe' with
-            | Except.ok _ => IO.println "Valid result"
-            | Except.error msg => IO.println ("Invalid result due to " ++ msg )
-        else
-          match checkValidnessMockDatabase problem with
-          | Except.error msg => IO.println ("Invalid result due to " ++ msg )
-          | Except.ok _ => IO.println "Valid result"
+      if argsParsed.graph = true
+      then
+        main_graph argsParsed
+      else
+        main_trees argsParsed
