CertifyingDatalog.lean
@@ -6,3 +6,4 @@ import «CertifyingDatalog».TreeValidation
 import «CertifyingDatalog».Unification
 import «CertifyingDatalog».Database
 import «CertifyingDatalog».ModelChecking
+import «CertifyingDatalog».GraphValidation
